ulib/FStar.Rational.fst
@@ -1,0 +1,571 @@
+(*
+   Copyright 2008-2026 Microsoft Research
+
+   Licensed under the Apache License, Version 2.0 (the "License");
+   you may not use this file except in compliance with the License.
+   You may obtain a copy of the License at
+
+       http://www.apache.org/licenses/LICENSE-2.0
+
+   Unless required by applicable law or agreed to in writing, software
+   distributed under the License is distributed on an "AS IS" BASIS,
+   WITHOUT WARRANTIES OR CONDITIONS OF ANY KIND, either express or implied.
+   See the License for the specific language governing permissions and
+   limitations under the License.
+*)
+module FStar.Rational
+
+open FStar.Rational.Gcd
+
+module L = FStar.Math.Lemmas
+
+#set-options "--fuel 0 --ifuel 0 --z3rlimit 20"
+
+let pmul a b = L.pos_times_pos_is_pos a b; a * b
+
+type frac = { n : int; d : pos }
+
+let rat = q:frac{ reduced q.n q.d }
+
+let num q = q.n
+let den q = q.d
+
+let mk (n:int) (d:pos) : rat =
+  reduce_ok n d;
+  let g = gcd n d in
+  { n = n / g; d = d / g }
+
+let frac_eta (q:frac) : Lemma ({ n = q.n; d = q.d } == q) =
+  match q with | { n = _; d = _ } -> ()
+
+(**** Representation lemmas *)
+
+let rearr_cross (a g b:int) : Lemma (a * (g * b) == (g * a) * b) = ()
+
+let mk_num_den (q:rat) : Lemma (mk (num q) (den q) == q) =
+  let g = gcd q.n q.d in
+  assert (g == 1);   // reduced q.n q.d
+  frac_eta q
+
+let num_den_reduced (q:rat) : Lemma (num q == 0 ==> den q == 1) =
+  introduce num q == 0 ==> den q == 1
+  with gcd_zero q.d
+
+let eq_cross (p q:rat)
+  : Lemma (p == q <==> num p * den q == num q * den p)
+  = introduce num p * den q == num q * den p ==> p == q
+    with begin
+      den_eq p.n p.d q.n q.d;             // p.d == q.d
+      L.lemma_cancel_mul p.n q.n p.d;     // p.n == q.n
+      frac_eta p;
+      frac_eta q
+    end
+
+let mk_cross (n:int) (d:pos)
+  : Lemma (num (mk n d) * d == n * den (mk n d))
+  = reduce_ok n d;
+    let g = gcd n d in
+    let a = n / g in
+    let b = d / g in
+    // num (mk n d) = a, den (mk n d) = b; n = g*a, d = g*b
+    rearr_cross a g b;   // a * (g * b) == (g * a) * b
+    assert (a * d == a * (g * b));
+    assert (n * b == (g * a) * b)
+
+let r1 (a b d1 d2:int) : Lemma ((a*b)*(d1*d2) == (a*d1)*(b*d2)) = ()
+let r2 (a b d1 d2:int) : Lemma ((a*b)*(d1*d2) == (a*d2)*(b*d1)) = ()
+let r3 (n b1 b2 d2:int) : Lemma ((n*b1)*(b2*d2) == (n*d2)*(b1*b2)) = ()
+let r4 (n b2 b1 d1:int) : Lemma ((n*b2)*(b1*d1) == (n*d1)*(b1*b2)) = ()
+
+let mk_eq_int (n1 d1 n2 d2 a1 b1 a2 b2:int)
+  : Lemma (requires d1>0 /\ d2>0 /\ b1>0 /\ b2>0 /\ a1*d1==n1*b1 /\ a2*d2==n2*b2)
+          (ensures (a1*b2==a2*b1) <==> (n1*d2==n2*d1))
+  = L.pos_times_pos_is_pos d1 d2;
+    L.pos_times_pos_is_pos b1 b2;
+    let x : pos = d1*d2 in
+    let y : pos = b1*b2 in
+    r1 a1 b2 d1 d2;
+    r3 n1 b1 b2 d2;
+    assert ((a1*b2)*x == (n1*d2)*y);
+    r2 a2 b1 d1 d2;
+    r4 n2 b2 b1 d1;
+    assert ((a2*b1)*x == (n2*d1)*y);
+    introduce a1*b2==a2*b1 ==> n1*d2==n2*d1
+    with L.lemma_cancel_mul (n1*d2) (n2*d1) y;
+    introduce n1*d2==n2*d1 ==> a1*b2==a2*b1
+    with L.lemma_cancel_mul (a1*b2) (a2*b1) x
+
+let mk_eq (n1:int) (d1:pos) (n2:int) (d2:pos)
+  : Lemma (mk n1 d1 == mk n2 d2 <==> n1 * d2 == n2 * d1)
+  = let p = mk n1 d1 in
+    let q = mk n2 d2 in
+    mk_cross n1 d1;
+    mk_cross n2 d2;
+    eq_cross p q;
+    mk_eq_int n1 d1 n2 d2 (num p) (den p) (num q) (den q)
+
+(**** Embedding of the integers *)
+
+let of_int (n:int) : rat = mk n 1
+
+let of_int_num_den (n:int) : Lemma (num (of_int n) == n /\ den (of_int n) == 1) =
+  reduced_den_one n   // gcd n 1 == 1, so n/1 == n and 1/1 == 1
+
+let of_int_mk (n:int) : Lemma (of_int n == mk n 1) = ()
+
+(**** Field operations *)
+
+let add p q = mk (num p * den q + num q * den p) (pmul (den p) (den q))
+let neg p = mk (- num p) (den p)
+let mul p q = mk (num p * num q) (pmul (den p) (den q))
+
+let inv p =
+  if num p = 0 then zero
+  else if num p > 0 then mk (den p) (num p)
+  else mk (- (den p)) (- (num p))
+
+(**** Order *)
+
+let lt p q = num p * den q < num q * den p
+
+(**** The mk congruences *)
+
+let dist_l (u v w:int) : Lemma ((u+v)*w == u*w + v*w) = ()
+
+let cross_step (a b d1 d2 n c:int)
+  : Lemma (requires a*d1 == n*c)
+          (ensures (a*b)*(d1*d2) == (n*d2)*(c*b))
+  = r1 a b d1 d2;    // (a*b)*(d1*d2) == (a*d1)*(b*d2)
+    r3 n c b d2      // (n*c)*(b*d2) == (n*d2)*(c*b)
+
+let cross_step2 (a b d1 d2 n c:int)
+  : Lemma (requires a*d2 == n*c)
+          (ensures (a*b)*(d1*d2) == (n*d1)*(b*c))
+  = r2 a b d1 d2;    // (a*b)*(d1*d2) == (a*d2)*(b*d1)
+    r4 n c b d1      // (n*c)*(b*d1) == (n*d1)*(b*c)
+
+let add_int (n1 d1 n2 d2 a1 b1 a2 b2:int)
+  : Lemma (requires a1*d1==n1*b1 /\ a2*d2==n2*b2)
+          (ensures (a1*b2+a2*b1)*(d1*d2) == (n1*d2+n2*d1)*(b1*b2))
+  = cross_step a1 b2 d1 d2 n1 b1;    // (a1*b2)*(d1*d2) == (n1*d2)*(b1*b2)
+    cross_step2 a2 b1 d1 d2 n2 b2;   // (a2*b1)*(d1*d2) == (n2*d1)*(b1*b2)
+    dist_l (a1*b2) (a2*b1) (d1*d2);
+    dist_l (n1*d2) (n2*d1) (b1*b2)
+
+let mk_add (n1:int) (d1:pos) (n2:int) (d2:pos)
+  : Lemma (add (mk n1 d1) (mk n2 d2) == mk (n1 * d2 + n2 * d1) (pmul d1 d2))
+  = let p = mk n1 d1 in
+    let q = mk n2 d2 in
+    mk_cross n1 d1;
+    mk_cross n2 d2;
+    add_int n1 d1 n2 d2 (num p) (den p) (num q) (den q);
+    mk_eq (num p * den q + num q * den p) (pmul (den p) (den q))
+          (n1 * d2 + n2 * d1) (pmul d1 d2)
+
+let neg_int (a d n b:int)
+  : Lemma (requires a*d==n*b) (ensures (-a)*d == (-n)*b)
+  = L.neg_mul_left a d;
+    L.neg_mul_left n b
+
+let mk_neg (n:int) (d:pos)
+  : Lemma (neg (mk n d) == mk (-n) d)
+  = let p = mk n d in
+    mk_cross n d;
+    neg_int (num p) d n (den p);
+    mk_eq (- num p) (den p) (-n) d
+
+let rm1 (a1 a2 d1 d2:int) : Lemma ((a1*a2)*(d1*d2) == (a1*d1)*(a2*d2)) = ()
+let rm2 (n1 b1 n2 b2:int) : Lemma ((n1*b1)*(n2*b2) == (n1*n2)*(b1*b2)) = ()
+
+let mul_int (n1 d1 n2 d2 a1 b1 a2 b2:int)
+  : Lemma (requires a1*d1==n1*b1 /\ a2*d2==n2*b2)
+          (ensures (a1*a2)*(d1*d2) == (n1*n2)*(b1*b2))
+  = rm1 a1 a2 d1 d2;
+    rm2 n1 b1 n2 b2
+
+let mk_mul (n1:int) (d1:pos) (n2:int) (d2:pos)
+  : Lemma (mul (mk n1 d1) (mk n2 d2) == mk (n1 * n2) (pmul d1 d2))
+  = let p = mk n1 d1 in
+    let q = mk n2 d2 in
+    mk_cross n1 d1;
+    mk_cross n2 d2;
+    mul_int n1 d1 n2 d2 (num p) (den p) (num q) (den q);
+    mk_eq (num p * num q) (pmul (den p) (den q)) (n1 * n2) (pmul d1 d2)
+
+let lt_mul_pos_iff (a:pos) (b c:int)
+  : Lemma (b*a < c*a <==> b < c)
+  = introduce b < c ==> b*a < c*a
+    with L.lemma_mult_lt_right a b c;
+    introduce b*a < c*a ==> b < c
+    with (if b < c then () else L.lemma_mult_le_right a c b)
+
+let mk_lt_int (n1 d1 n2 d2 a1 b1 a2 b2:int)
+  : Lemma (requires d1>0 /\ d2>0 /\ b1>0 /\ b2>0 /\ a1*d1==n1*b1 /\ a2*d2==n2*b2)
+          (ensures (a1*b2 < a2*b1) <==> (n1*d2 < n2*d1))
+  = L.pos_times_pos_is_pos d1 d2;
+    L.pos_times_pos_is_pos b1 b2;
+    let x : pos = d1*d2 in
+    let y : pos = b1*b2 in
+    r1 a1 b2 d1 d2;
+    r3 n1 b1 b2 d2;
+    assert ((a1*b2)*x == (n1*d2)*y);
+    r2 a2 b1 d1 d2;
+    r4 n2 b2 b1 d1;
+    assert ((a2*b1)*x == (n2*d1)*y);
+    lt_mul_pos_iff x (a1*b2) (a2*b1);
+    lt_mul_pos_iff y (n1*d2) (n2*d1)
+
+let mk_lt (n1:int) (d1:pos) (n2:int) (d2:pos)
+  : Lemma (lt (mk n1 d1) (mk n2 d2) <==> n1 * d2 < n2 * d1)
+  = let p = mk n1 d1 in
+    let q = mk n2 d2 in
+    mk_cross n1 d1;
+    mk_cross n2 d2;
+    mk_lt_int n1 d1 n2 d2 (num p) (den p) (num q) (den q)
+
+(**** Inverse *)
+
+let inv_num_den (q:rat)
+  : Lemma (requires q =!= zero) (ensures mul q (inv q) == one)
+  = mk_num_den q;
+    of_int_num_den 0;
+    frac_eta zero;
+    if num q = 0 then begin
+      num_den_reduced q;
+      frac_eta q  // q == {n=0;d=1} == zero, contradicting precondition
+    end
+    else if num q > 0 then begin
+      assert (inv q == mk (den q) (num q));
+      mk_mul (num q) (den q) (den q) (num q);
+      of_int_mk 1;
+      mk_eq (num q * den q) (pmul (den q) (num q)) 1 1
+    end
+    else begin
+      assert (inv q == mk (- (den q)) (- (num q)));
+      mk_mul (num q) (den q) (- (den q)) (- (num q));
+      of_int_mk 1;
+      mk_eq (num q * (- (den q))) (pmul (den q) (- (num q))) 1 1
+    end
+
+(**** Additive laws *)
+
+let add_comm (p q:rat) : Lemma (add p q == add q p) =
+  mk_num_den p; mk_num_den q;
+  mk_add (num p) (den p) (num q) (den q);
+  mk_add (num q) (den q) (num p) (den p);
+  mk_eq (num p * den q + num q * den p) (pmul (den p) (den q))
+        (num q * den p + num p * den q) (pmul (den q) (den p))
+
+let t1 (a e g:int) : Lemma ((a*e)*g == a*(e*g)) = ()
+let t2 (c b g:int) : Lemma ((c*b)*g == (c*g)*b) = ()
+let t3 (f b e:int) : Lemma (f*(b*e) == (f*e)*b) = ()
+let assoc_num (a b c e f g:int)
+  : Lemma ((a*e+c*b)*g + f*(b*e) == a*(e*g) + (c*g+f*e)*b)
+  = dist_l (a*e) (c*b) g;
+    dist_l (c*g) (f*e) b;
+    t1 a e g; t2 c b g; t3 f b e
+let assoc_den (b e g:int) : Lemma ((b*e)*g == b*(e*g)) = ()
+
+let add_assoc (p q r:rat) : Lemma (add (add p q) r == add p (add q r)) =
+  let a = num p in let b = den p in
+  let c = num q in let e = den q in
+  let f = num r in let g = den r in
+  mk_num_den p; mk_num_den q; mk_num_den r;
+  mk_add a b c e;                       // add p q == mk (a*e+c*b) (b*e)
+  mk_add c e f g;                       // add q r == mk (c*g+f*e) (e*g)
+  mk_add (a*e+c*b) (pmul b e) f g;
+  mk_add a b (c*g+f*e) (pmul e g);
+  assoc_num a b c e f g;
+  assoc_den b e g;
+  mk_eq ((a*e+c*b)*g + f*(pmul b e)) (pmul (pmul b e) g)
+        (a*(pmul e g) + (c*g+f*e)*b) (pmul b (pmul e g))
+
+let add_zero (p:rat) : Lemma (add p zero == p) =
+  mk_num_den p;
+  of_int_mk 0;                          // zero == mk 0 1
+  mk_add (num p) (den p) 0 1;
+  mk_eq (num p * 1 + 0 * den p) (pmul (den p) 1) (num p) (den p)
+
+let add_neg (p:rat) : Lemma (add p (neg p) == zero) =
+  mk_num_den p;
+  mk_neg (num p) (den p);               // neg p == mk (-(num p)) (den p)
+  mk_add (num p) (den p) (- num p) (den p);
+  of_int_mk 0;
+  L.neg_mul_left (num p) (den p);
+  mk_eq (num p * den p + (- num p) * den p) (pmul (den p) (den p)) 0 1
+
+let neg_neg (p:rat) : Lemma (neg (neg p) == p) =
+  mk_num_den p;
+  mk_neg (num p) (den p);               // neg p == mk (-(num p)) (den p)
+  mk_neg (- num p) (den p);             // neg (neg p) == mk (- - num p) (den p)
+  mk_eq (- (- num p)) (den p) (num p) (den p)
+
+(**** Multiplicative laws *)
+
+let mul_comm (p q:rat) : Lemma (mul p q == mul q p) =
+  mk_num_den p; mk_num_den q;
+  mk_mul (num p) (den p) (num q) (den q);
+  mk_mul (num q) (den q) (num p) (den p);
+  mk_eq (num p * num q) (pmul (den p) (den q))
+        (num q * num p) (pmul (den q) (den p))
+
+let mul_assoc (p q r:rat) : Lemma (mul (mul p q) r == mul p (mul q r)) =
+  let a = num p in let b = den p in
+  let c = num q in let e = den q in
+  let f = num r in let g = den r in
+  mk_num_den p; mk_num_den q; mk_num_den r;
+  mk_mul a b c e;
+  mk_mul c e f g;
+  mk_mul (a*c) (pmul b e) f g;
+  mk_mul a b (c*f) (pmul e g);
+  t1 a c f;                            // (a*c)*f == a*(c*f)
+  assoc_den b e g;                     // (b*e)*g == b*(e*g)
+  mk_eq ((a*c)*f) (pmul (pmul b e) g) (a*(c*f)) (pmul b (pmul e g))
+
+let mul_one (p:rat) : Lemma (mul p one == p) =
+  mk_num_den p;
+  of_int_mk 1;
+  mk_mul (num p) (den p) 1 1;
+  mk_eq (num p * 1) (pmul (den p) 1) (num p) (den p)
+
+let mul_zero (p:rat) : Lemma (mul p zero == zero) =
+  mk_num_den p;
+  of_int_mk 0;
+  mk_mul (num p) (den p) 0 1;
+  mk_eq (num p * 0) (pmul (den p) 1) 0 1
+
+let mul_neg (p q:rat) : Lemma (mul (neg p) q == neg (mul p q)) =
+  mk_num_den p; mk_num_den q;
+  mk_neg (num p) (den p);
+  mk_mul (- num p) (den p) (num q) (den q);
+  mk_mul (num p) (den p) (num q) (den q);
+  mk_neg (num p * num q) (pmul (den p) (den q));
+  L.neg_mul_left (num p) (num q);
+  mk_eq ((- num p) * num q) (pmul (den p) (den q))
+        (- (num p * num q)) (pmul (den p) (den q))
+
+(**** Distributivity *)
+
+let scale_cross (k n d:int) : Lemma ((k*n)*d == n*(k*d)) = ()
+
+let mk_scale (k:pos) (n:int) (d:pos)
+  : Lemma (mk (k*n) (pmul k d) == mk n d)
+  = scale_cross k n d;
+    mk_eq (k*n) (pmul k d) n d
+
+let dist_r (w u v:int) : Lemma (w*(u+v) == w*u + w*v) = ()
+let m4 (a b c g:int) : Lemma ((a*c)*(b*g) == b*(a*(c*g))) = ()
+let rd4 (b e g:int) : Lemma ((b*e)*(b*g) == b*(b*(e*g))) = ()
+
+let dist_rn (a b c e f g:int)
+  : Lemma ((a*c)*(b*g) + (a*f)*(b*e) == b*(a*(c*g+f*e)))
+  = m4 a b c g;                 // (a*c)*(b*g) == b*(a*(c*g))
+    m4 a b f e;                 // (a*f)*(b*e) == b*(a*(f*e))
+    dist_r a (c*g) (f*e);       // a*(c*g+f*e) == a*(c*g) + a*(f*e)
+    dist_r b (a*(c*g)) (a*(f*e))// b*(x+y) == b*x + b*y
+
+let distrib (p q r:rat) : Lemma (mul p (add q r) == add (mul p q) (mul p r)) =
+  let a = num p in let b = den p in
+  let c = num q in let e = den q in
+  let f = num r in let g = den r in
+  mk_num_den p; mk_num_den q; mk_num_den r;
+  mk_add c e f g;                          // add q r == mk (c*g+f*e) (e*g)
+  mk_mul a b (c*g+f*e) (pmul e g);         // LHS == mk (a*(c*g+f*e)) (b*(e*g))
+  mk_mul a b c e;                          // mul p q == mk (a*c) (b*e)
+  mk_mul a b f g;                          // mul p r == mk (a*f) (b*g)
+  mk_add (a*c) (pmul b e) (a*f) (pmul b g);// RHS == mk ((a*c)*(b*g)+(a*f)*(b*e)) ((b*e)*(b*g))
+  let nd : pos = pmul b (pmul e g) in      // = b*(e*g), the LHS denominator
+  dist_rn a b c e f g;                     // RHSnum == b*(a*(c*g+f*e))
+  rd4 b e g;                               // RHSden == b*nd
+  mk_scale b (a*(c*g+f*e)) nd              // mk (b*N) (pmul b nd) == mk N nd
+
+let mul_eq_zero (p q:rat)
+  : Lemma (mul p q == zero <==> (p == zero \/ q == zero))
+  = mk_num_den p; mk_num_den q;
+    mk_mul (num p) (den p) (num q) (den q);
+    of_int_mk 0;
+    mk_eq (num p * num q) (pmul (den p) (den q)) 0 1;
+    mk_eq (num p) (den p) 0 1;
+    mk_eq (num q) (den q) 0 1
+
+(**** Order laws *)
+
+let swp (x y z:int) : Lemma ((x*y)*z == (x*z)*y) = ()
+
+let lt_irrefl (p:rat) : Lemma (~(lt p p)) = ()
+
+let lt_trans_int (a b c e f g:int)
+  : Lemma (requires b>0 /\ e>0 /\ g>0 /\ a*e<c*b /\ c*g<f*e)
+          (ensures  a*g<f*b)
+  = L.lemma_mult_lt_right g (a*e) (c*b);   // (a*e)*g < (c*b)*g
+    L.lemma_mult_lt_right b (c*g) (f*e);   // (c*g)*b < (f*e)*b
+    t2 c b g;                              // (c*b)*g == (c*g)*b
+    swp a e g;                             // (a*e)*g == (a*g)*e
+    swp f e b;                             // (f*e)*b == (f*b)*e
+    lt_mul_pos_iff e (a*g) (f*b)
+
+let lt_trans (p q r:rat) : Lemma (requires lt p q /\ lt q r) (ensures lt p r) =
+  lt_trans_int (num p) (den p) (num q) (den q) (num r) (den r)
+
+let lt_total (p q:rat) : Lemma (lt p q \/ p == q \/ lt q p) =
+  eq_cross p q
+
+let lt_asym (p q:rat) : Lemma (requires lt p q) (ensures ~(lt q p)) = ()
+
+let mm1 (a g e:int) : Lemma ((a*g)*(e*g) == (a*e)*(g*g)) = ()
+let mm2 (c g b:int) : Lemma ((c*g)*(b*g) == (c*b)*(g*g)) = ()
+let seq (f e b g:int) : Lemma ((f*e)*(b*g) == (f*b)*(e*g)) = ()
+
+let lt_add_r_int (a b c e f g:int)
+  : Lemma (requires b>0 /\ e>0 /\ g>0)
+          (ensures ((a*g+f*b)*(e*g) < (c*g+f*e)*(b*g)) <==> (a*e < c*b))
+  = L.pos_times_pos_is_pos g g;
+    let gg : pos = g*g in
+    dist_l (a*g) (f*b) (e*g);   // (a*g+f*b)*(e*g) == (a*g)*(e*g)+(f*b)*(e*g)
+    dist_l (c*g) (f*e) (b*g);   // (c*g+f*e)*(b*g) == (c*g)*(b*g)+(f*e)*(b*g)
+    mm1 a g e;                  // (a*g)*(e*g) == (a*e)*gg
+    mm2 c g b;                  // (c*g)*(b*g) == (c*b)*gg
+    seq f e b g;                // (f*e)*(b*g) == (f*b)*(e*g)
+    lt_mul_pos_iff gg (a*e) (c*b)
+
+let lt_add_r (p q r:rat) : Lemma (lt (add p r) (add q r) <==> lt p q) =
+  mk_lt (num p * den r + num r * den p) (pmul (den p) (den r))
+        (num q * den r + num r * den q) (pmul (den q) (den r));
+  lt_add_r_int (num p) (den p) (num q) (den q) (num r) (den r)
+
+let lt_neg (p q:rat) : Lemma (lt (neg q) (neg p) <==> lt p q) =
+  mk_num_den p; mk_num_den q;
+  mk_neg (num p) (den p);
+  mk_neg (num q) (den q);
+  mk_lt (- num q) (den q) (- num p) (den p);
+  L.neg_mul_left (num q) (den p);
+  L.neg_mul_left (num p) (den q)
+
+let hkm (x h y k:int) : Lemma ((x*h)*(y*k) == (x*y)*(h*k)) = ()
+
+let lt_mul_pos_int (a b c e h k:int)
+  : Lemma (requires b>0 /\ e>0 /\ h>0 /\ k>0)
+          (ensures ((a*h)*(e*k) < (c*h)*(b*k)) <==> (a*e < c*b))
+  = L.pos_times_pos_is_pos h k;
+    let hk : pos = h*k in
+    hkm a h e k;                 // (a*h)*(e*k) == (a*e)*hk
+    hkm c h b k;                 // (c*h)*(b*k) == (c*b)*hk
+    lt_mul_pos_iff hk (a*e) (c*b)
+
+let lt_mul_pos (p q r:rat)
+  : Lemma (requires lt zero r) (ensures lt (mul p r) (mul q r) <==> lt p q)
+  = of_int_num_den 0;
+    mk_lt (num p * num r) (pmul (den p) (den r))
+          (num q * num r) (pmul (den q) (den r));
+    lt_mul_pos_int (num p) (den p) (num q) (den q) (num r) (den r)
+
+let mul_pos (p q:rat)
+  : Lemma (requires lt zero p /\ lt zero q) (ensures lt zero (mul p q))
+  = of_int_num_den 0;
+    of_int_mk 0;
+    mk_mul (num p) (den p) (num q) (den q);
+    mk_lt 0 1 (num p * num q) (pmul (den p) (den q))
+
+let inv_pos (p:rat)
+  : Lemma (requires lt zero p) (ensures lt zero (inv p))
+  = of_int_num_den 0;
+    assert (inv p == mk (den p) (num p));
+    of_int_mk 0;
+    mk_lt 0 1 (den p) (num p)
+
+(**** Integers, floor, Archimedes, density *)
+
+let of_int_add (m n:int) : Lemma (of_int (m + n) == add (of_int m) (of_int n)) =
+  of_int_mk m; of_int_mk n; of_int_mk (m+n);
+  mk_add m 1 n 1;
+  mk_eq (m*1 + n*1) (pmul 1 1) (m+n) 1
+
+let of_int_mul (m n:int) : Lemma (of_int (m * n) == mul (of_int m) (of_int n)) =
+  of_int_mk m; of_int_mk n; of_int_mk (m*n);
+  mk_mul m 1 n 1;
+  mk_eq (m*n) (pmul 1 1) (m*n) 1
+
+let of_int_lt (m n:int) : Lemma (lt (of_int m) (of_int n) <==> m < n) =
+  of_int_mk m; of_int_mk n;
+  mk_lt m 1 n 1
+
+let of_int_inj (m n:int) : Lemma (of_int m == of_int n <==> m == n) =
+  of_int_mk m; of_int_mk n;
+  mk_eq m 1 n 1
+
+let floor (q:rat) : int = num q / den q
+
+let floor_spec (q:rat)
+  : Lemma (le (of_int (floor q)) q /\ lt q (of_int (floor q + 1)))
+  = let a = num q in let b = den q in
+    mk_num_den q;
+    of_int_mk (floor q);
+    of_int_mk (floor q + 1);
+    L.lemma_div_mod a b;      // a == b*(a/b) + a%b
+    L.lemma_mod_lt a b;       // 0 <= a%b < b
+    mk_lt (floor q) 1 a b;    // lt (of_int (floor q)) q <==> (floor q)*b < a
+    mk_eq (floor q) 1 a b;    // of_int (floor q) == q <==> (floor q)*b == a
+    mk_lt a b (floor q + 1) 1 // lt q (of_int (floor q + 1)) <==> a < (floor q + 1)*b
+
+let archimedean (q:rat) : Lemma (exists (n:nat). lt q (of_int n)) =
+  let a = num q in let b = den q in
+  mk_num_den q;
+  let m : nat = if a <= 0 then 1 else a + 1 in
+  of_int_mk m;
+  mk_lt a b m 1;                    // lt q (of_int m) <==> a < m*b
+  L.lemma_mult_le_left m 1 b;       // m*1 <= m*b  (since 1 <= b)
+  introduce exists (n:nat). lt q (of_int n) with m and ()
+
+let small_inv (eps:rat)
+  : Lemma (requires lt zero eps) (ensures exists (n:pos). lt (mk 1 n) eps)
+  = let a = num eps in let b = den eps in
+    mk_num_den eps;
+    of_int_num_den 0;               // 0 < a
+    let m : pos = b + 1 in
+    mk_lt 1 m a b;                  // lt (mk 1 m) eps <==> b < a*m
+    L.lemma_mult_le_right m 1 a;    // 1*m <= a*m  (since 1 <= a)
+    introduce exists (n:pos). lt (mk 1 n) eps with m and ()
+
+let mid (p q:rat) : rat =
+  mk (num p * den q + num q * den p) (pmul (pmul (den p) (den q)) 2)
+
+let q1 (a b e:int) : Lemma (a*((b*e)*2) == (a*e)*b + (a*e)*b) = ()
+let q2 (c b e:int) : Lemma (c*((b*e)*2) == (c*b)*e + (c*b)*e) = ()
+
+let mid_lo (a b c e:int)
+  : Lemma (requires b>0 /\ e>0)
+          (ensures (a*((b*e)*2) < (a*e+c*b)*b) <==> (a*e < c*b))
+  = q1 a b e;
+    dist_l (a*e) (c*b) b;
+    lt_mul_pos_iff b (a*e) (c*b)
+
+let mid_hi (a b c e:int)
+  : Lemma (requires b>0 /\ e>0)
+          (ensures ((a*e+c*b)*e < c*((b*e)*2)) <==> (a*e < c*b))
+  = dist_l (a*e) (c*b) e;
+    q2 c b e;
+    lt_mul_pos_iff e (a*e) (c*b)
+
+let mid_spec (p q:rat)
+  : Lemma (requires lt p q) (ensures lt p (mid p q) /\ lt (mid p q) q)
+  = let a = num p in let b = den p in
+    let c = num q in let e = den q in
+    mk_num_den p; mk_num_den q;
+    mk_lt a b (a*e+c*b) (pmul (pmul b e) 2);
+    mk_lt (a*e+c*b) (pmul (pmul b e) 2) c e;
+    mid_lo a b c e;
+    mid_hi a b c e
+
+let below (q:rat) : r:rat{lt r q} =
+  let a = num q in let b = den q in
+  mk_num_den q;
+  mk_lt (a - b) b a b;
+  lt_mul_pos_iff b (a - b) a;
+  mk (a - b) b
+
+let above (q:rat) : r:rat{lt q r} =
+  let a = num q in let b = den q in
+  mk_num_den q;
+  mk_lt a b (a + b) b;
+  lt_mul_pos_iff b a (a + b);
+  mk (a + b) b
