ulib/FStar.Real.Dedekind.Add.fst
@@ -1,0 +1,542 @@
+(*
+   Copyright 2008-2026 Microsoft Research
+
+   Licensed under the Apache License, Version 2.0 (the "License");
+   you may not use this file except in compliance with the License.
+   You may obtain a copy of the License at
+
+       http://www.apache.org/licenses/LICENSE-2.0
+
+   Unless required by applicable law or agreed to in writing, software
+   distributed under the License is distributed on an "AS IS" BASIS,
+   WITHOUT WARRANTIES OR CONDITIONS OF ANY KIND, either express or implied.
+   See the License for the specific language governing permissions and
+   limitations under the License.
+*)
+module FStar.Real.Dedekind.Add
+
+/// The additive group of Dedekind cuts.
+///
+///   x + y  =  { a + b       | a in x, b in y }
+///     - x  =  { q | exists r > 0. -q - r not in x }
+///
+/// The offset [r] in the definition of negation is what stops [-x] from having
+/// a greatest element when [x] is the cut of a rational.
+///
+/// Nothing is assumed here; see [FStar.Real.Dedekind.Base] for the (purely
+/// logical) axioms the development rests on.
+
+module Q = FStar.Rational
+module B = FStar.Real.Dedekind.Base
+module ID = FStar.IndefiniteDescription
+
+#set-options "--fuel 0 --ifuel 0 --z3rlimit 20"
+
+(**** Rational helpers *)
+
+/// Each of these is stated on its own: batching them, or reasoning about them
+/// inside a larger proof, is markedly slower.
+
+let qlt_add2 (a a' b b':Q.rat)
+  : Lemma (requires Q.lt a a' /\ Q.lt b b')
+          (ensures Q.lt (Q.add a b) (Q.add a' b'))
+  = Q.lt_add_r a a' b;
+    Q.lt_add_r b b' a';
+    Q.add_comm b a'; Q.add_comm b' a';
+    Q.lt_trans (Q.add a b) (Q.add a' b) (Q.add a' b')
+
+let qlt_add_l (a a' b:Q.rat)
+  : Lemma (Q.lt (Q.add b a) (Q.add b a') <==> Q.lt a a')
+  = Q.lt_add_r a a' b; Q.add_comm b a; Q.add_comm b a'
+
+let qadd_zero_l (q:Q.rat) : Lemma (Q.add Q.zero q == q)
+  = Q.add_comm Q.zero q; Q.add_zero q
+
+let qsub_add (q b:Q.rat) : Lemma (Q.add (Q.sub q b) b == q)
+  = Q.add_assoc q (Q.neg b) b;
+    Q.add_comm (Q.neg b) b;
+    Q.add_neg b;
+    Q.add_comm b (Q.neg b);
+    Q.add_zero q
+
+let qadd_sub (b q:Q.rat) : Lemma (Q.add b (Q.sub q b) == q)
+  = qsub_add q b; Q.add_comm b (Q.sub q b)
+
+let qadd_sub_cancel (a b:Q.rat) : Lemma (Q.sub (Q.add a b) b == a)
+  = Q.add_assoc a b (Q.neg b); Q.add_neg b; Q.add_zero a
+
+let qsub_lt (q q' b:Q.rat)
+  : Lemma (Q.lt (Q.sub q' b) (Q.sub q b) <==> Q.lt q' q)
+  = Q.lt_add_r q' q (Q.neg b)
+
+let qneg_add (a b:Q.rat) : Lemma (Q.neg (Q.add a b) == Q.add (Q.neg a) (Q.neg b))
+  = Q.mul_neg Q.one (Q.add a b);
+    Q.mul_comm Q.one (Q.add a b); Q.mul_one (Q.add a b);
+    Q.distrib (Q.neg Q.one) a b;
+    Q.mul_comm (Q.neg Q.one) a; Q.mul_neg Q.one a;
+    Q.mul_comm Q.one a; Q.mul_one a;
+    Q.mul_comm (Q.neg Q.one) b; Q.mul_neg Q.one b;
+    Q.mul_comm Q.one b; Q.mul_one b
+
+let qneg_zero () : Lemma (Q.neg Q.zero == Q.zero)
+  = Q.add_neg Q.zero; qadd_zero_l (Q.neg Q.zero)
+
+let qneg_lt_zero (q:Q.rat) : Lemma (Q.lt Q.zero (Q.neg q) <==> Q.lt q Q.zero)
+  = qneg_zero (); Q.lt_neg q Q.zero
+
+(**** Addition *)
+
+let addp (x y:B.cut) (q:Q.rat) : prop =
+  exists (a b:Q.rat). x a /\ y b /\ q == Q.add a b
+
+let add_ne (x y:B.cut) : Lemma (exists (q:Q.rat). addp x y q)
+  = let a = B.cut_mem x in
+    let b = B.cut_mem y in
+    introduce exists (q:Q.rat). addp x y q with (Q.add a b) and ()
+
+let add_nf (x y:B.cut) : Lemma (exists (q:Q.rat). ~(addp x y q))
+  = let a' = B.cut_nonmem x in
+    let b' = B.cut_nonmem y in
+    introduce addp x y (Q.add a' b') ==> False
+    with eliminate exists (a b:Q.rat). x a /\ y b /\ Q.add a' b' == Q.add a b
+      with begin
+        B.mem_lt_nonmem x a a';
+        B.mem_lt_nonmem y b b';
+        qlt_add2 a a' b b';
+        Q.lt_irrefl (Q.add a b)
+      end;
+    introduce exists (q:Q.rat). ~(addp x y q) with (Q.add a' b') and ()
+
+let add_dc (x y:B.cut)
+  : Lemma (forall (u v:Q.rat). (addp x y v /\ Q.lt u v) ==> addp x y u)
+  = introduce forall (u v:Q.rat). (addp x y v /\ Q.lt u v) ==> addp x y u
+    with introduce _ ==> _ with
+      eliminate exists (a b:Q.rat). x a /\ y b /\ v == Q.add a b
+      with begin
+        qsub_add u b;
+        qadd_sub_cancel a b;
+        qsub_lt v u b;
+        B.cut_down x (Q.sub u b) a;
+        introduce exists (a2 b2:Q.rat). x a2 /\ y b2 /\ u == Q.add a2 b2
+        with (Q.sub u b) b and ()
+      end
+
+let add_op (x y:B.cut)
+  : Lemma (forall (u:Q.rat). addp x y u ==>
+                        (exists (v:Q.rat). addp x y v /\ Q.lt u v))
+  = introduce forall (u:Q.rat). addp x y u ==>
+                           (exists (v:Q.rat). addp x y v /\ Q.lt u v)
+    with introduce _ ==> _ with
+      eliminate exists (a b:Q.rat). x a /\ y b /\ u == Q.add a b
+      with begin
+        let a2 = B.cut_above x a in
+        Q.lt_add_r a a2 b;
+        introduce exists (v:Q.rat). addp x y v /\ Q.lt u v
+        with (Q.add a2 b) and ()
+      end
+
+let cadd (x y:B.cut) : c:B.cut{forall (q:Q.rat). c q <==> addp x y q} =
+  add_ne x y; add_nf x y; add_dc x y; add_op x y;
+  B.mk_cut (addp x y)
+
+(**** Negation *)
+
+let oppp (x:B.cut) (q:Q.rat) : prop =
+  exists (r:Q.rat). Q.lt Q.zero r /\ ~(x (Q.neg (Q.add q r)))
+
+let opp_ne (x:B.cut) : Lemma (exists (q:Q.rat). oppp x q)
+  = let b = B.cut_nonmem x in
+    let q = Q.neg (Q.add b Q.one) in
+    Q.of_int_lt 0 1;
+    qneg_add b Q.one;
+    Q.neg_neg b; Q.neg_neg Q.one;
+    Q.add_assoc (Q.neg b) (Q.neg Q.one) Q.one;
+    Q.add_comm (Q.neg Q.one) Q.one;
+    Q.add_neg Q.one;
+    Q.add_comm Q.one (Q.neg Q.one);
+    Q.add_zero (Q.neg b);
+    qneg_add (Q.neg b) (Q.neg Q.one);
+    introduce exists (r:Q.rat). Q.lt Q.zero r /\ ~(x (Q.neg (Q.add q r)))
+    with Q.one and ();
+    introduce exists (q:Q.rat). oppp x q with q and ()
+
+let opp_nf (x:B.cut) : Lemma (exists (q:Q.rat). ~(oppp x q))
+  = let a = B.cut_mem x in
+    introduce oppp x (Q.neg a) ==> False
+    with eliminate exists (r:Q.rat). Q.lt Q.zero r /\
+                             ~(x (Q.neg (Q.add (Q.neg a) r)))
+      with begin
+        qneg_add (Q.neg a) r;
+        Q.neg_neg a;
+        Q.lt_add_r Q.zero r (Q.neg r);
+        Q.add_neg r;
+        qadd_zero_l (Q.neg r);
+        qlt_add_l (Q.neg r) Q.zero a;
+        Q.add_zero a;
+        B.cut_down x (Q.add a (Q.neg r)) a
+      end;
+    introduce exists (q:Q.rat). ~(oppp x q) with (Q.neg a) and ()
+
+let opp_dc (x:B.cut)
+  : Lemma (forall (u v:Q.rat). (oppp x v /\ Q.lt u v) ==> oppp x u)
+  = introduce forall (u v:Q.rat). (oppp x v /\ Q.lt u v) ==> oppp x u
+    with introduce _ ==> _ with
+      eliminate exists (r:Q.rat). Q.lt Q.zero r /\ ~(x (Q.neg (Q.add v r)))
+      with begin
+        let s = Q.add r (Q.sub v u) in
+        qsub_lt v u u;
+        Q.add_neg u;
+        qlt_add_l Q.zero (Q.sub v u) r;
+        Q.add_zero r;
+        Q.lt_trans Q.zero r s;
+        Q.add_assoc u r (Q.sub v u);
+        Q.add_comm r (Q.sub v u);
+        Q.add_assoc u (Q.sub v u) r;
+        qadd_sub u v;
+        introduce exists (r:Q.rat). Q.lt Q.zero r /\ ~(x (Q.neg (Q.add u r)))
+        with s and ()
+      end
+
+let opp_op (x:B.cut)
+  : Lemma (forall (u:Q.rat). oppp x u ==>
+                        (exists (v:Q.rat). oppp x v /\ Q.lt u v))
+  = introduce forall (u:Q.rat). oppp x u ==>
+                           (exists (v:Q.rat). oppp x v /\ Q.lt u v)
+    with introduce _ ==> _ with
+      eliminate exists (r:Q.rat). Q.lt Q.zero r /\ ~(x (Q.neg (Q.add u r)))
+      with begin
+        let s = Q.mid Q.zero r in
+        Q.mid_spec Q.zero r;
+        let v = Q.add u (Q.sub r s) in
+        qsub_lt r s s;
+        Q.add_neg s;
+        qlt_add_l Q.zero (Q.sub r s) u;
+        Q.add_zero u;
+        Q.add_assoc u (Q.sub r s) s;
+        qsub_add r s;
+        introduce exists (r:Q.rat). Q.lt Q.zero r /\ ~(x (Q.neg (Q.add v r)))
+        with s and ();
+        introduce exists (v:Q.rat). oppp x v /\ Q.lt u v with v and ()
+      end
+
+#push-options "--z3rlimit 200"
+let copp (x:B.cut) : c:B.cut{forall (q:Q.rat). c q <==> oppp x q} =
+  opp_ne x; opp_nf x; opp_dc x; opp_op x;
+  B.mk_cut (oppp x)
+#pop-options
+
+(**** More rational rearrangements *)
+
+let ac_shuffle (p q r:Q.rat)
+  : Lemma (Q.add (Q.add p q) r == Q.add (Q.add p r) q)
+  = Q.add_assoc p q r; Q.add_comm q r; Q.add_assoc p r q
+
+let qadd_neg_l (b:Q.rat) : Lemma (Q.add (Q.neg b) b == Q.zero)
+  = Q.add_neg b; Q.add_comm b (Q.neg b)
+
+/// [(-(b+r)) + b == -r]
+let qcancel2 (b r:Q.rat)
+  : Lemma (Q.add (Q.neg (Q.add b r)) b == Q.neg r)
+  = qneg_add b r;
+    ac_shuffle (Q.neg b) (Q.neg r) b;
+    qadd_neg_l b;
+    qadd_zero_l (Q.neg r)
+
+/// [-((-(a+r)) + r) == a]
+let qcancel1 (a r:Q.rat)
+  : Lemma (Q.neg (Q.add (Q.neg (Q.add a r)) r) == a)
+  = qneg_add a r;
+    Q.add_assoc (Q.neg a) (Q.neg r) r;
+    qadd_neg_l r;
+    Q.add_zero (Q.neg a);
+    Q.neg_neg a
+
+/// [a + (-((a+e)+r)) == -(e+r)]
+let qcancel3 (a e r:Q.rat)
+  : Lemma (Q.add a (Q.neg (Q.add (Q.add a e) r)) == Q.neg (Q.add e r))
+  = Q.add_assoc a e r;
+    qneg_add a (Q.add e r);
+    Q.add_assoc a (Q.neg a) (Q.neg (Q.add e r));
+    Q.add_neg a;
+    qadd_zero_l (Q.neg (Q.add e r))
+
+let qneg_lt_zero' (r:Q.rat) : Lemma (Q.lt (Q.neg r) Q.zero <==> Q.lt Q.zero r)
+  = qneg_zero (); Q.lt_neg Q.zero r
+
+(**** Commutativity *)
+
+let cadd_comm_sub (x y:B.cut) : Lemma (B.cle (cadd x y) (cadd y x))
+  = introduce forall (q:Q.rat). cadd x y q ==> cadd y x q
+    with introduce _ ==> _ with
+      eliminate exists (a b:Q.rat). x a /\ y b /\ q == Q.add a b
+      with begin
+        Q.add_comm a b;
+        introduce exists (a2 b2:Q.rat). y a2 /\ x b2 /\ q == Q.add a2 b2
+        with b a and ()
+      end
+
+let cadd_comm (x y:B.cut) : Lemma (cadd x y == cadd y x)
+  = cadd_comm_sub x y; cadd_comm_sub y x;
+    B.cle_antisym (cadd x y) (cadd y x)
+
+(**** Associativity *)
+
+let cadd_assoc_sub (x y z:B.cut)
+  : Lemma (B.cle (cadd (cadd x y) z) (cadd x (cadd y z)))
+  = introduce forall (q:Q.rat). cadd (cadd x y) z q ==> cadd x (cadd y z) q
+    with introduce _ ==> _ with
+      eliminate exists (u c:Q.rat). cadd x y u /\ z c /\ q == Q.add u c
+      with eliminate exists (a b:Q.rat). x a /\ y b /\ u == Q.add a b
+      with begin
+        Q.add_assoc a b c;
+        introduce exists (b2 c2:Q.rat). y b2 /\ z c2 /\ Q.add b c == Q.add b2 c2
+        with b c and ();
+        introduce exists (a2 u2:Q.rat). x a2 /\ cadd y z u2 /\ q == Q.add a2 u2
+        with a (Q.add b c) and ()
+      end
+
+let cadd_assoc_sub' (x y z:B.cut)
+  : Lemma (B.cle (cadd x (cadd y z)) (cadd (cadd x y) z))
+  = introduce forall (q:Q.rat). cadd x (cadd y z) q ==> cadd (cadd x y) z q
+    with introduce _ ==> _ with
+      eliminate exists (a u:Q.rat). x a /\ cadd y z u /\ q == Q.add a u
+      with eliminate exists (b c:Q.rat). y b /\ z c /\ u == Q.add b c
+      with begin
+        Q.add_assoc a b c;
+        introduce exists (a2 b2:Q.rat). x a2 /\ y b2 /\ Q.add a b == Q.add a2 b2
+        with a b and ();
+        introduce exists (u2 c2:Q.rat). cadd x y u2 /\ z c2 /\ q == Q.add u2 c2
+        with (Q.add a b) c and ()
+      end
+
+let cadd_assoc (x y z:B.cut)
+  : Lemma (cadd (cadd x y) z == cadd x (cadd y z))
+  = cadd_assoc_sub x y z; cadd_assoc_sub' x y z;
+    B.cle_antisym (cadd (cadd x y) z) (cadd x (cadd y z))
+
+(**** Zero *)
+
+let czero : B.cut = B.rat_cut Q.zero
+
+let cadd_zero_sub (x:B.cut) : Lemma (B.cle (cadd x czero) x)
+  = introduce forall (q:Q.rat). cadd x czero q ==> x q
+    with introduce _ ==> _ with
+      eliminate exists (a b:Q.rat). x a /\ czero b /\ q == Q.add a b
+      with begin
+        B.rat_cut_mem Q.zero b;
+        qlt_add_l b Q.zero a;
+        Q.add_zero a;
+        B.cut_down x q a
+      end
+
+let cadd_zero_sub' (x:B.cut) : Lemma (B.cle x (cadd x czero))
+  = introduce forall (q:Q.rat). x q ==> cadd x czero q
+    with introduce _ ==> _ with begin
+      let a = B.cut_above x q in
+      qsub_lt a q a;
+      Q.add_neg a;
+      B.rat_cut_mem Q.zero (Q.sub q a);
+      qadd_sub a q;
+      introduce exists (a2 b2:Q.rat). x a2 /\ czero b2 /\ q == Q.add a2 b2
+      with a (Q.sub q a) and ()
+    end
+
+let cadd_zero (x:B.cut) : Lemma (cadd x czero == x)
+  = cadd_zero_sub x; cadd_zero_sub' x;
+    B.cle_antisym (cadd x czero) x
+
+(**** Inverses *)
+
+let cadd_opp_sub (x:B.cut) : Lemma (B.cle (cadd x (copp x)) czero)
+  = introduce forall (q:Q.rat). cadd x (copp x) q ==> czero q
+    with introduce _ ==> _ with
+      eliminate exists (a b:Q.rat). x a /\ copp x b /\ q == Q.add a b
+      with eliminate exists (r:Q.rat). Q.lt Q.zero r /\ ~(x (Q.neg (Q.add b r)))
+      with begin
+        B.mem_lt_nonmem x a (Q.neg (Q.add b r));
+        Q.lt_add_r a (Q.neg (Q.add b r)) b;
+        qcancel2 b r;
+        qneg_lt_zero' r;
+        Q.lt_trans q (Q.neg r) Q.zero;
+        B.rat_cut_mem Q.zero q
+      end
+
+let cadd_opp_sub' (x:B.cut) : Lemma (B.cle czero (cadd x (copp x)))
+  = introduce forall (q:Q.rat). czero q ==> cadd x (copp x) q
+    with introduce _ ==> _ with begin
+      B.rat_cut_mem Q.zero q;
+      qneg_lt_zero q;
+      let e = Q.mid Q.zero (Q.neg q) in
+      Q.mid_spec Q.zero (Q.neg q);
+      let r = Q.sub (Q.neg q) e in
+      qsub_lt (Q.neg q) e e;
+      Q.add_neg e;
+      let ab = B.approx x e in
+      let a = fst ab in
+      let a' = snd ab in
+      let b = Q.neg (Q.add a' r) in
+      qcancel1 a' r;
+      introduce exists (r2:Q.rat). Q.lt Q.zero r2 /\ ~(x (Q.neg (Q.add b r2)))
+      with r and ();
+      qcancel3 a e r;
+      qadd_sub e (Q.neg q);
+      Q.neg_neg q;
+      introduce exists (a2 b2:Q.rat). x a2 /\ copp x b2 /\ q == Q.add a2 b2
+      with a b and ()
+    end
+
+let cadd_opp (x:B.cut) : Lemma (cadd x (copp x) == czero)
+  = cadd_opp_sub x; cadd_opp_sub' x;
+    B.cle_antisym (cadd x (copp x)) czero
+
+(**** Compatibility of addition with the order *)
+
+let qshift (q q2 c:Q.rat)
+  : Lemma (Q.add q (Q.add c (Q.sub q2 q)) == Q.add q2 c)
+  = Q.add_comm c (Q.sub q2 q);
+    Q.add_assoc q (Q.sub q2 q) c;
+    qadd_sub q q2
+
+let cadd_mono (x y z:B.cut)
+  : Lemma (requires B.clt x y) (ensures B.clt (cadd x z) (cadd y z))
+  = let q = B.clt_witness x y in
+    let q2 = B.cut_above y q in
+    let e = Q.sub q2 q in
+    qsub_lt q2 q q;
+    Q.add_neg q;
+    let cc = B.approx z e in
+    let c = fst cc in
+    let c' = snd cc in
+    let w = Q.add q2 c in
+    introduce exists (a2 b2:Q.rat). y a2 /\ z b2 /\ w == Q.add a2 b2
+    with q2 c and ();
+    introduce cadd x z w ==> False
+    with eliminate exists (a b:Q.rat). x a /\ z b /\ w == Q.add a b
+    with begin
+      B.mem_lt_nonmem x a q;
+      B.mem_lt_nonmem z b c';
+      qlt_add2 a q b c';
+      qshift q q2 c;
+      Q.lt_irrefl w
+    end;
+    B.clt_of_witness (cadd x z) (cadd y z) w
+
+let cadd_mono_rev (x y z:B.cut)
+  : Lemma (B.clt (cadd x z) (cadd y z) <==> B.clt x y)
+  = introduce B.clt x y ==> B.clt (cadd x z) (cadd y z)
+    with cadd_mono x y z;
+    introduce B.clt (cadd x z) (cadd y z) ==> B.clt x y
+    with begin
+      B.clt_total x y;
+      B.clt_irrefl (cadd x z);
+      introduce B.clt y x ==> B.clt x y
+      with begin
+        cadd_mono y x z;
+        B.clt_trans (cadd x z) (cadd y z) (cadd x z);
+        B.clt_irrefl (cadd x z)
+      end
+    end
+
+(**** The embedding is additive *)
+
+let qsub_flip (t a q:Q.rat)
+  : Lemma (Q.lt (Q.sub t a) q <==> Q.lt (Q.sub t q) a)
+  = Q.lt_add_r (Q.sub t a) q (Q.sub a q);
+    qadd_sub q a;
+    Q.add_assoc (Q.sub t a) a (Q.neg q);
+    qsub_add t a
+
+let rat_add_sub (p q:Q.rat)
+  : Lemma (B.cle (B.rat_cut (Q.add p q)) (cadd (B.rat_cut p) (B.rat_cut q)))
+  = introduce forall (t:Q.rat).
+        B.rat_cut (Q.add p q) t ==> cadd (B.rat_cut p) (B.rat_cut q) t
+    with introduce _ ==> _ with begin
+      B.rat_cut_mem (Q.add p q) t;
+      qsub_add t q;
+      Q.lt_add_r (Q.sub t q) p q;
+      let a = Q.mid (Q.sub t q) p in
+      Q.mid_spec (Q.sub t q) p;
+      let b = Q.sub t a in
+      qsub_flip t a q;
+      qadd_sub a t;
+      B.rat_cut_mem p a;
+      B.rat_cut_mem q b;
+      introduce exists (a2 b2:Q.rat).
+          B.rat_cut p a2 /\ B.rat_cut q b2 /\ t == Q.add a2 b2
+      with a b and ()
+    end
+
+let rat_add_sub' (p q:Q.rat)
+  : Lemma (B.cle (cadd (B.rat_cut p) (B.rat_cut q)) (B.rat_cut (Q.add p q)))
+  = introduce forall (t:Q.rat).
+        cadd (B.rat_cut p) (B.rat_cut q) t ==> B.rat_cut (Q.add p q) t
+    with introduce _ ==> _ with
+      eliminate exists (a b:Q.rat).
+          B.rat_cut p a /\ B.rat_cut q b /\ t == Q.add a b
+      with begin
+        B.rat_cut_mem p a;
+        B.rat_cut_mem q b;
+        qlt_add2 a p b q;
+        B.rat_cut_mem (Q.add p q) t
+      end
+
+let rat_add (p q:Q.rat)
+  : Lemma (B.rat_cut (Q.add p q) == cadd (B.rat_cut p) (B.rat_cut q))
+  = rat_add_sub p q; rat_add_sub' p q;
+    B.cle_antisym (B.rat_cut (Q.add p q)) (cadd (B.rat_cut p) (B.rat_cut q))
+
+(**** The embedding respects negation *)
+
+let qneg_lt (t p:Q.rat) : Lemma (Q.lt t (Q.neg p) <==> Q.lt p (Q.neg t))
+  = Q.lt_neg t (Q.neg p); Q.neg_neg p;
+    Q.lt_neg p (Q.neg t); Q.neg_neg t
+
+let rat_opp_sub (p:Q.rat)
+  : Lemma (B.cle (B.rat_cut (Q.neg p)) (copp (B.rat_cut p)))
+  = introduce forall (t:Q.rat). B.rat_cut (Q.neg p) t ==> copp (B.rat_cut p) t
+    with introduce _ ==> _ with begin
+      B.rat_cut_mem (Q.neg p) t;
+      qneg_lt t p;
+      let r = Q.mid Q.zero (Q.sub (Q.neg t) p) in
+      qsub_lt (Q.neg t) p p;
+      Q.add_neg p;
+      Q.mid_spec Q.zero (Q.sub (Q.neg t) p);
+      qsub_add (Q.neg t) p;
+      Q.lt_add_r r (Q.sub (Q.neg t) p) p;
+      Q.add_comm r p;
+      Q.lt_add_r (Q.add p r) (Q.neg t) (Q.neg r);
+      Q.add_assoc p r (Q.neg r);
+      Q.add_neg r;
+      Q.add_zero p;
+      qneg_add t r;
+      B.rat_cut_mem p (Q.neg (Q.add t r));
+      Q.lt_asym p (Q.neg (Q.add t r));
+      introduce exists (r2:Q.rat).
+          Q.lt Q.zero r2 /\ ~(B.rat_cut p (Q.neg (Q.add t r2)))
+      with r and ()
+    end
+
+let rat_opp_sub' (p:Q.rat)
+  : Lemma (B.cle (copp (B.rat_cut p)) (B.rat_cut (Q.neg p)))
+  = introduce forall (t:Q.rat). copp (B.rat_cut p) t ==> B.rat_cut (Q.neg p) t
+    with introduce _ ==> _ with
+      eliminate exists (r:Q.rat).
+          Q.lt Q.zero r /\ ~(B.rat_cut p (Q.neg (Q.add t r)))
+      with begin
+        B.rat_cut_mem p (Q.neg (Q.add t r));
+        qneg_add t r;
+        qneg_lt_zero' r;
+        Q.lt_add_r (Q.neg r) Q.zero (Q.neg t);
+        qadd_zero_l (Q.neg t);
+        Q.add_comm (Q.neg t) (Q.neg r);
+        Q.lt_total p (Q.neg (Q.add t r));
+        introduce Q.lt p (Q.neg (Q.add t r)) ==> Q.lt p (Q.neg t)
+        with Q.lt_trans p (Q.neg (Q.add t r)) (Q.neg t);
+        qneg_lt t p;
+        B.rat_cut_mem (Q.neg p) t
+      end
+
+let rat_opp (p:Q.rat)
+  : Lemma (B.rat_cut (Q.neg p) == copp (B.rat_cut p))
+  = rat_opp_sub p; rat_opp_sub' p;
+    B.cle_antisym (B.rat_cut (Q.neg p)) (copp (B.rat_cut p))
