ulib/FStar.Real.Ordered.fst
@@ -1,0 +1,344 @@
+(*
+   Copyright 2008-2026 Microsoft Research
+
+   Licensed under the Apache License, Version 2.0 (the "License");
+   you may not use this file except in compliance with the License.
+   You may obtain a copy of the License at
+
+       http://www.apache.org/licenses/LICENSE-2.0
+
+   Unless required by applicable law or agreed to in writing, software
+   distributed under the License is distributed on an "AS IS" BASIS,
+   WITHOUT WARRANTIES OR CONDITIONS OF ANY KIND, either express or implied.
+   See the License for the specific language governing permissions and
+   limitations under the License.
+*)
+module FStar.Real.Ordered
+
+open FStar.Real.Dedekind
+
+module Q = FStar.Rational
+module ID = FStar.IndefiniteDescription
+
+#set-options "--fuel 0 --ifuel 0 --z3rlimit 20"
+
+(**** Order *)
+
+let lt_asym (x y:real) : Lemma (requires lt x y) (ensures ~(lt y x))
+  = lt_irrefl x;
+    introduce lt y x ==> False with lt_trans x y x
+
+let not_lt (x y:real) : Lemma (~(lt x y) <==> le y x)
+  = lt_irrefl x; lt_irrefl y; lt_total x y;
+    introduce lt y x ==> ~(lt x y) with lt_asym y x;
+    introduce lt x y ==> ~(le y x) with lt_asym x y
+
+let le_refl (x:real) : Lemma (le x x) = ()
+
+let le_trans (x y z:real)
+  : Lemma (requires le x y /\ le y z) (ensures le x z)
+  = introduce (lt x y /\ lt y z) ==> lt x z with lt_trans x y z
+
+let lt_le_trans (x y z:real)
+  : Lemma (requires lt x y /\ le y z) (ensures lt x z)
+  = introduce lt y z ==> lt x z with lt_trans x y z
+
+let le_lt_trans (x y z:real)
+  : Lemma (requires le x y /\ lt y z) (ensures lt x z)
+  = introduce lt x y ==> lt x z with lt_trans x y z
+
+let le_antisym (x y:real)
+  : Lemma (requires le x y /\ le y x) (ensures x == y)
+  = introduce (lt x y /\ lt y x) ==> x == y with lt_asym x y
+
+(**** Additive group *)
+
+let add_zero_l (x:real) : Lemma (add zero x == x)
+  = add_comm zero x; add_zero x
+
+let add_opp_l (x:real) : Lemma (add (opp x) x == zero)
+  = add_comm (opp x) x; add_opp x
+
+let add_cancel (x y z:real) : Lemma (add x z == add y z <==> x == y)
+  = add_assoc x z (opp z); add_assoc y z (opp z);
+    add_opp z; add_zero x; add_zero y
+
+let opp_opp (x:real) : Lemma (opp (opp x) == x)
+  = add_opp (opp x);
+    add_comm (opp x) (opp (opp x));
+    add_opp x;
+    add_cancel (opp (opp x)) x (opp x)
+
+let opp_zero () : Lemma (opp zero == zero)
+  = add_opp zero; add_zero_l (opp zero)
+
+/// [(a+b) + (c+d) == (a+c) + (b+d)]
+let shuffle4 (a b c d:real)
+  : Lemma (add (add a b) (add c d) == add (add a c) (add b d))
+  = add_assoc a b (add c d);
+    add_assoc b c d; add_comm b c; add_assoc c b d;
+    add_assoc a c (add b d)
+
+let opp_add (x y:real) : Lemma (opp (add x y) == add (opp x) (opp y))
+  = shuffle4 (opp x) (opp y) x y;
+    add_opp_l x; add_opp_l y; add_zero zero;
+    add_opp_l (add x y);
+    add_cancel (add (opp x) (opp y)) (opp (add x y)) (add x y)
+
+let sub_self (x:real) : Lemma (sub x x == zero) = add_opp x
+
+let sub_add (x y:real) : Lemma (add (sub x y) y == x)
+  = add_assoc x (opp y) y; add_opp_l y; add_zero x
+
+let add_sub (x y:real) : Lemma (sub (add x y) y == x)
+  = add_assoc x y (opp y); add_opp y; add_zero x
+
+let lt_add_l (x y z:real) : Lemma (lt (add z x) (add z y) <==> lt x y)
+  = lt_add_r x y z; add_comm z x; add_comm z y
+
+let le_add_r (x y z:real) : Lemma (le (add x z) (add y z) <==> le x y)
+  = lt_add_r x y z; add_cancel x y z
+
+let lt_sub (x y:real) : Lemma (lt x y <==> lt zero (sub y x))
+  = lt_add_r zero (sub y x) x; add_zero_l x; sub_add y x
+
+let le_sub (x y:real) : Lemma (le x y <==> le zero (sub y x))
+  = le_add_r zero (sub y x) x; add_zero_l x; sub_add y x
+
+let lt_opp (x y:real) : Lemma (lt (opp y) (opp x) <==> lt x y)
+  = lt_add_r (opp y) (opp x) (add x y);
+    add_comm (opp y) (add x y);
+    add_assoc x y (opp y); add_opp y; add_zero x;
+    add_assoc (opp x) x y; add_opp_l x; add_zero_l y
+
+let lt_add_compat (a b c d:real)
+  : Lemma (requires lt a b /\ le c d) (ensures lt (add a c) (add b d))
+  = lt_add_r a b c;
+    le_add_r c d b; add_comm c b; add_comm d b;
+    lt_le_trans (add a c) (add b c) (add b d)
+
+(**** Multiplication *)
+
+let mul_zero_l (x:real) : Lemma (mul zero x == zero)
+  = mul_comm zero x; mul_zero x
+
+let mul_one_l (x:real) : Lemma (mul one x == x)
+  = mul_comm one x; mul_one x
+
+let distrib_r (x y z:real) : Lemma (mul (add x y) z == add (mul x z) (mul y z))
+  = mul_comm (add x y) z; distrib z x y; mul_comm z x; mul_comm z y
+
+let mul_opp (x y:real) : Lemma (mul (opp x) y == opp (mul x y))
+  = distrib_r (opp x) x y; add_opp_l x; mul_zero_l y;
+    add_opp_l (mul x y);
+    add_cancel (mul (opp x) y) (opp (mul x y)) (mul x y)
+
+let mul_opp_r (x y:real) : Lemma (mul x (opp y) == opp (mul x y))
+  = mul_comm x (opp y); mul_opp y x; mul_comm y x
+
+let mul_sub (x y z:real) : Lemma (mul x (sub y z) == sub (mul x y) (mul x z))
+  = distrib x y (opp z); mul_opp_r x z
+
+let mul_sub_r (x y z:real) : Lemma (mul (sub x y) z == sub (mul x z) (mul y z))
+  = distrib_r x (opp y) z; mul_opp y z
+
+let mul_pos (x y:real)
+  : Lemma (requires lt zero x /\ lt zero y) (ensures lt zero (mul x y))
+  = lt_mul_pos zero x y; mul_zero_l y
+
+let mul_nonneg (x y:real)
+  : Lemma (requires le zero x /\ le zero y) (ensures le zero (mul x y))
+  = mul_zero_l y; mul_zero x;
+    introduce (lt zero x /\ lt zero y) ==> lt zero (mul x y)
+    with mul_pos x y
+
+let le_mul_pos (x y z:real)
+  : Lemma (requires lt zero z) (ensures le (mul x z) (mul y z) <==> le x y)
+  = lt_mul_pos x y z; lt_mul_pos y x z; lt_total x y;
+    lt_irrefl (mul x z); lt_irrefl (mul y z)
+
+let mul_lt_compat (a b c d:real)
+  : Lemma (requires le zero a /\ lt a b /\ le zero c /\ lt c d)
+          (ensures  lt (mul a c) (mul b d))
+  = le_lt_trans zero a b;
+    le_lt_trans zero c d;
+    lt_mul_pos c d b; mul_comm c b; mul_comm d b;
+    mul_zero a; mul_zero b; le_refl zero;
+    introduce lt zero c ==> le (mul a c) (mul b c)
+    with le_mul_pos a b c;
+    le_lt_trans (mul a c) (mul b c) (mul b d)
+
+let mul_le_compat (a b c d:real)
+  : Lemma (requires le zero a /\ le a b /\ le zero c /\ le c d)
+          (ensures  le (mul a c) (mul b d))
+  = le_trans zero a b;
+    mul_zero a; mul_zero b; mul_zero_l c; mul_zero_l d;
+    le_refl zero; le_refl (mul b c);
+    introduce lt zero c ==> le (mul a c) (mul b c)
+    with le_mul_pos a b c;
+    introduce lt zero b ==> le (mul c b) (mul d b)
+    with le_mul_pos c d b;
+    mul_comm c b; mul_comm d b;
+    le_trans (mul a c) (mul b c) (mul b d)
+
+(**** Squares *)
+
+let sq_nonneg (x:real)
+  : Lemma (requires le zero x) (ensures le zero (mul x x))
+  = mul_nonneg x x
+
+let sq_mono (x y:real)
+  : Lemma (requires le zero x /\ lt x y) (ensures lt (mul x x) (mul y y))
+  = mul_lt_compat x y x y
+
+let sq_mono_rev (x y:real)
+  : Lemma (requires le zero x /\ le zero y /\ lt (mul x x) (mul y y))
+          (ensures  lt x y)
+  = not_lt x y;
+    introduce le y x ==> False
+    with begin
+      mul_le_compat y x y x;
+      not_lt (mul x x) (mul y y)
+    end
+
+let sq_inj (x y:real)
+  : Lemma (requires le zero x /\ le zero y /\ mul x x == mul y y)
+          (ensures  x == y)
+  = lt_total x y; lt_irrefl (mul x x);
+    introduce lt x y ==> False with sq_mono x y;
+    introduce lt y x ==> False with sq_mono y x
+
+/// [two == one + one], needed before its own [val] appears in the interface.
+let two_eq_aux () : Lemma (two == add one one)
+  = Q.of_int_add 1 1; of_rat_add (Q.of_int 1) (Q.of_int 1)
+
+let two_mul (a:real) : Lemma (mul two a == add a a)
+  = two_eq_aux (); distrib_r one one a; mul_one_l a
+
+let square_add (x y:real)
+  : Lemma (mul (add x y) (add x y) ==
+           add (add (mul x x) (mul two (mul x y))) (mul y y))
+  = distrib_r x y (add x y);
+    distrib x x y; distrib y x y;
+    mul_comm y x;
+    two_mul (mul x y);
+    add_assoc (mul x x) (mul x y) (add (mul x y) (mul y y));
+    add_assoc (mul x y) (mul x y) (mul y y);
+    add_assoc (mul x x) (add (mul x y) (mul x y)) (mul y y)
+
+let square_sub (x y:real)
+  : Lemma (mul (sub x y) (sub x y) ==
+           add (sub (mul x x) (mul two (mul x y))) (mul y y))
+  = square_add x (opp y);
+    mul_opp_r x y;
+    mul_opp_r two (mul x y);
+    mul_opp y (opp y);
+    mul_opp_r y y;
+    opp_opp (mul y y)
+
+(**** Constants and inverses *)
+
+let zero_lt_one () : Lemma (lt zero one)
+  = Q.of_int_lt 0 1; of_rat_lt (Q.of_int 0) (Q.of_int 1)
+
+let zero_lt_two () : Lemma (lt zero two)
+  = Q.of_int_lt 0 2; of_rat_lt (Q.of_int 0) (Q.of_int 2)
+
+let two_eq () : Lemma (two == add one one) = two_eq_aux ()
+
+let one_ne_zero () : Lemma (one =!= zero)
+  = Q.of_int_inj 1 0; of_rat_inj (Q.of_int 1) (Q.of_int 0)
+
+let inv_pos (x:real)
+  : Lemma (requires lt zero x) (ensures lt zero (inv x))
+  = lt_irrefl zero; zero_lt_one (); one_ne_zero ();
+    mul_inv x;
+    lt_total zero (inv x);
+    mul_zero x;
+    lt_mul_pos (inv x) zero x; mul_zero_l x; mul_comm (inv x) x;
+    lt_asym zero one
+
+let inv_antitone (x y:real)
+  : Lemma (requires lt zero x /\ lt x y) (ensures lt (inv y) (inv x))
+  = lt_trans zero x y;
+    inv_pos x; inv_pos y;
+    mul_pos (inv x) (inv y);
+    lt_mul_pos x y (mul (inv x) (inv y));
+    lt_irrefl zero;
+    mul_inv x; mul_inv y;
+    mul_assoc x (inv x) (inv y);
+    mul_comm (inv x) (inv y);
+    mul_assoc y (inv y) (inv x);
+    mul_one_l (inv y); mul_one_l (inv x)
+
+let div_pos (x y:real)
+  : Lemma (requires lt zero x /\ lt zero y) (ensures lt zero (div x y))
+  = inv_pos y; mul_pos x (inv y)
+
+let mul_div (x y:real)
+  : Lemma (requires y =!= zero) (ensures mul (div x y) y == x)
+  = mul_assoc x (inv y) y; mul_comm (inv y) y; mul_inv y; mul_one x
+
+let div_lt_iff (x y z:real)
+  : Lemma (requires lt zero z) (ensures lt (div x z) y <==> lt x (mul y z))
+  = lt_irrefl zero; mul_div x z; lt_mul_pos (div x z) y z
+
+let of_rat_inv (q:Q.rat)
+  : Lemma (requires q =!= Q.zero) (ensures inv (of_rat q) == of_rat (Q.inv q))
+  = Q.inv_num_den q;
+    of_rat_inj q Q.zero;
+    of_rat_mul q (Q.inv q);
+    mul_inv (of_rat q);
+    mul_one (of_rat (Q.inv q));
+    mul_assoc (of_rat (Q.inv q)) (of_rat q) (inv (of_rat q));
+    mul_comm (of_rat (Q.inv q)) (of_rat q);
+    mul_one_l (inv (of_rat q))
+
+(**** Density of the rationals; smallness *)
+
+/// [1/(1/x) == x]
+let inv_inv (x:real)
+  : Lemma (requires x =!= zero /\ inv x =!= zero)
+          (ensures inv (inv x) == x)
+  = mul_inv x; mul_inv (inv x);
+    mul_one x;
+    mul_assoc x (inv x) (inv (inv x));
+    mul_one_l (inv (inv x))
+
+let small_rat (u:real)
+  : Ghost Q.rat (requires lt zero u)
+                (ensures fun q -> Q.lt Q.zero q /\ lt zero (of_rat q) /\
+                               lt (of_rat q) u)
+  = inv_pos u;
+    lt_irrefl zero;
+    archimedean (inv u);
+    let n = ID.indefinite_description_ghost nat
+              (fun n -> lt (inv u) (of_int n)) in
+    (* n > 0, since 0 < 1/u < n *)
+    lt_trans zero (inv u) (of_int n);
+    of_rat_lt (Q.of_int 0) (Q.of_int n);
+    Q.of_int_lt 0 n;
+    (* 1/n < 1/(1/u) == u *)
+    inv_antitone (inv u) (of_int n);
+    inv_inv u;
+    Q.inv_pos (Q.of_int n);
+    Q.of_int_lt 0 n;
+    Q.lt_irrefl Q.zero;
+    of_rat_inj (Q.of_int n) Q.zero;
+    Q.of_int_inj n 0;
+    of_rat_inv (Q.of_int n);
+    of_rat_lt Q.zero (Q.inv (Q.of_int n));
+    Q.inv (Q.of_int n)
+
+let small_pos (u:real)
+  : Ghost real (requires lt zero u) (ensures fun e -> lt zero e /\ lt e u)
+  = of_rat (small_rat u)
+
+let small_pos2 (u v:real)
+  : Ghost real (requires lt zero u /\ lt zero v)
+               (ensures fun e -> lt zero e /\ lt e u /\ lt e v)
+  = let e1 = small_pos u in
+    let e2 = small_pos v in
+    if ID.strong_excluded_middle (lt e1 e2)
+    then (lt_trans e1 e2 v; e1)
+    else (not_lt e1 e2; le_lt_trans e2 e1 u; e2)
